src/Comparse.Tactic.fst
@@ -2,5 +2,5 @@ module Comparse.Tactic
 
 include Comparse.Tactic.Attributes
 include Comparse.Tactic.GenerateParser
-include Comparse.Tactic.GenerateIsValidLemma
+include Comparse.Tactic.GenerateIsWellFormedLemma
 include Comparse.Tactic.GenerateLengthLemma
